priorities attempt

TreapNode.dfy
@@ -9,6 +9,8 @@ class TreapNode {
   ghost var Repr: set<TreapNode>
   // Needed to check for BST property
   ghost var Values: set<int>
+  // Needed to check for heap property
+  ghost var Priorities: set<int>
 
   ghost predicate Valid()
     reads this, Repr
@@ -18,24 +20,45 @@ class TreapNode {
          && left in Repr
          && this !in left.Repr
          && left.Repr <= Repr
+         && priority !in left.Priorities
+         && left.Priorities <= Priorities
          && left.Valid()
-         && forall x :: x in left.Values ==> x < key  // BST property
-                        )
+         && (forall x :: x in left.Values ==> x < key)  // BST property
+                         )
     && ( right != null ==>
          && right in Repr
          && this !in right.Repr
          && right.Repr <= Repr
+         && priority !in right.Priorities
+         && right.Priorities <= Priorities
          && right.Valid()
-         && forall x :: x in right.Values ==> x > key  // BST property
+         && (forall x :: x in right.Values ==> x > key)  // BST property
+                         )
+    && // Extra check to ensure only one path between 2 nodes.
+       (right != null && left != null ==>
+         (forall x :: x in left.Repr ==> x !in right.Repr) && (forall y :: y in left.Priorities ==> y !in right.Priorities))
+    && ((left == null && right == null) ==> Values == {key} && Priorities == {priority})
+    && ((left != null && right == null) ==> Values == {key} + left.Values && Priorities == {priority} + left.Priorities)
+    && ((left == null && right != null) ==> Values == {key} + right.Values && Priorities == {priority} + right.Priorities)
+    && ((left != null && right != null) ==> Values == {key} + left.Values + right.Values && Priorities == {priority} + left.Priorities + right.Priorities)
+  }
+
+  ghost predicate ValidHeap()
+    reads this, Repr
+  {
+    && Valid()
+    && ( left != null ==>
+         && left.ValidHeap()
+         && forall x :: x in left.Priorities ==> x < priority  // Heap property
                         )
-    && ( // Extra check to ensure only one path between 2 nodes.
-       (right != null && left != null) ==>
-         ((forall x :: x in left.Repr ==> x !in right.Repr) &&
-                       (forall y :: y in right.Repr ==> y !in left.Repr)))
-    && ((left == null && right == null) ==> Values == {key})
-    && ((left != null && right == null) ==> Values == {key} + left.Values)
-    && ((left == null && right != null) ==> Values == {key} + right.Values)
-    && ((left != null && right != null) ==> Values == {key} + left.Values + right.Values)
+    && ( right != null ==>
+         && right.ValidHeap()
+         && forall x :: x in right.Priorities ==> x < priority  // Heap property
+                        )
+       // && ((left == null && right == null) ==> Priorities == {priority})
+       // && ((left != null && right == null) ==> Priorities == {priority} + left.Priorities)
+       // && ((left == null && right != null) ==> Priorities == {priority} + right.Priorities)
+       // && ((left != null && right != null) ==> Priorities == {priority} + left.Priorities + right.Priorities)
   }
 
   predicate IsLeaf()
@@ -49,6 +72,7 @@ class TreapNode {
     ensures Valid()
     ensures Repr == {this}
     ensures Values == {key}
+    ensures Priorities == {priority}
     ensures fresh(Repr)
   {
     this.key := key;
@@ -57,5 +81,6 @@ class TreapNode {
     this.right := null;
     Repr := {this};
     Values := {key};
+    Priorities := {priority};
   }
 }
